Finish extracting the (ab)* parser

src/Parsers/Refinement/SharpenedABStar.v
@@ -5,7 +5,7 @@ Set Implicit Arguments.
 
 Section IndexedImpl.
 
-  Lemma ComputationalSplitter
+  Lemma ComputationalSplitter'
   : FullySharpened (string_spec ab_star_grammar).
   Proof.
     start honing parser using indexed representation.
@@ -19,6 +19,14 @@ Section IndexedImpl.
     FullySharpenEachMethodWithoutDelegation.
     extract delegate-free implementation.
     simpl; higher_order_reflexivityT.
+  Defined.
+
+  Lemma ComputationalSplitter
+  : FullySharpened (string_spec ab_star_grammar).
+  Proof.
+    let impl := (eval simpl in (projT1 ComputationalSplitter')) in
+    refine (existT _ impl _).
+    abstract (exact (projT2 ComputationalSplitter')).
   Defined.
 
 End IndexedImpl.
@@ -53,275 +61,23 @@ Local Arguments string_dec : simpl never.
 Local Arguments Equality.string_beq : simpl never.
 Arguments SplitterFromParserADT.msplits / .
 Arguments splits_for / .
+Arguments Equality.ascii_beq !_ !_ / .
+Arguments SplitterFromParserADT.mlength / .
+Arguments SplitterFromParserADT.mis_char / .
+Arguments SplitterFromParserADT.mtake / .
+Arguments SplitterFromParserADT.mdrop / .
+Arguments SplitterFromParserADT.mto_string / .
+Arguments new_string_of_string / .
+Arguments ComputationalSplitter / .
+Arguments ComputationalADT.cRep / .
+Arguments new_string_of_base_string / .
+Arguments ComputationalADT.cConstructors / .
 Local Notation hextr0 := (ex _).
 Local Notation exist' x := (exist _ x _).
 Local Notation hextr1 := (or_intror _).
 Local Notation hextr2 := (or_introl _).
 
-Definition ab_star_parser' (str : String.string) : bool.
-Proof.
-  pose (has_parse (parser ComputationalSplitter) str) as impl.
-  Timeout 2 cbv beta iota zeta delta [has_parse parser ParserImplementationOptimized.parser transfer_parser List.fold_right] in impl.
-  repeat (let impl' := (eval cbv delta [impl] in impl) in
-          match impl' with
-            | appcontext G[fst (?x, _)] => let G' := context G[x] in change impl' with G' in impl
-            | appcontext G[snd (_, ?x)] => let G' := context G[x] in change impl' with G' in impl
-          end).
-  Timeout 2 cbv beta iota zeta delta [List.map List.hd List.fold_left item_ascii_cons item_of_char item_of_string] in impl.
-  repeat (let impl' := (eval cbv delta [impl] in impl) in
-          match impl' with
-            | appcontext G[fst (?x, _)] => let G' := context G[x] in change impl' with G' in impl
-            | appcontext G[snd (_, ?x)] => let G' := context G[x] in change impl' with G' in impl
-          end).
-  Timeout 2 cbv beta iota zeta delta [BooleanRecognizer.parse_production BooleanRecognizer.parse_item BooleanBaseTypes.split_string_for_production parser_data ParserImplementation.parser_data new_string_of_string] in impl.
-  change (orb false) with (fun x : bool => x) in impl.
-  cbv beta in impl.
-  change (@StringLike.String Ascii.ascii (ParserInterface.string_type
-                                            (SplitterFromParserADT.adt_based_splitter
-                                               ComputationalSplitter)))
-  with ({ r : (String.string * (nat * nat)) | exists orig, AbsR (projT2 ComputationalSplitter) orig r }%type)
-    in impl.
-  Timeout 2 change ((@StringLike.length _ (ParserInterface.string_type
-                                             (SplitterFromParserADT.adt_based_splitter
-                                                ComputationalSplitter))))
-  with (fun str : { r : (String.string * (nat * nat)) | exists orig, AbsR (projT2 ComputationalSplitter) orig r }%type => ilength (` str)) in impl.
-  do_simpl_in (Valid_nonterminals ab_star_grammar) impl.
-  Timeout 2 change (new_string_of_base_string ComputationalSplitter str)
-  with (str, (0, String.length str)) in impl.
-  Timeout 2 cbv beta iota zeta in impl.
-  Timeout 2 cbv beta iota zeta delta [splits_for] in impl.
-  Timeout 2 cbv beta iota zeta delta [is_char string_type splits_for SplitterFromParserADT.adt_based_splitter] in impl.
-  Timeout 2 cbv beta iota zeta delta [SplitterFromParserADT.msplits ComputationalADT.cMethods ComputationalADT.pcMethods] in impl.
-  Timeout 2 match eval cbv delta [impl] in impl with
-              | context[@projT2 ?A ?B (@projT1 ?C ?D ComputationalSplitter)]
-                => set_subst_hnf_in (@projT2 A B (@projT1 C D ComputationalSplitter)) impl
-            end.
-  Timeout 2 cbv beta iota zeta delta [BuildComputationalADT.getcMethDef BuildComputationalADT.cMethBody] in impl.
-(** HERE *)
-Locate StringBound.ith_Bounded.
-Print StringBound.ith_Bounded.
-Print StringBound.BoundedIndex.
-Print StringBound.IndexBound.
+Time Definition ab_star_parser (str : String.string) : bool
+  := Eval simpl in has_parse (parser ComputationalSplitter) str.
 
-  Timeout 2 let H := fresh in
-            set (H := (projT2 (projT1 ComputationalSplitter))) in impl;
-              hnf in H;
-              subst H.
-
-  let
-  Timeout 2 set_subst_hnf_in (projT2 (projT1 ComputationalSplitter)) impl.
-  hnf in X.
-  Timeout 2 subst X.
-  Opaque AbsR.
-  Timeout 2 pose (sf := (splits_for
-                         (SplitterFromParserADT.adt_based_splitter
-                            ComputationalSplitter))).
-  hnf in sf.
-  Set Printing Implicit.
-  Opaque StringLike.String SplitterFromParserADT.adt_based_StringLike AbsR.
-  Opaque ComputationalSplitter.
-  Timeout 2 simpl in impl.
-  Transparent SplitterFromParserADT.adt_based_StringLike.
-  Timeout 2 simpl in impl.
-  Arguments SplitterFromParserADT.mis_char / .
-  Timeout 2 simpl in impl.
-  Unset Printing Implicit.
-  Transparent ComputationalSplitter.
-  Arguments ComputationalADT.cMethodType / .
-  Arguments ComputationalADT.cMethods / .
-  Arguments If_Then_Else / .
-  repeat (let impl' := (eval cbv delta [impl] in impl) in
-          match impl' with
-            | appcontext G[ComputationalADT.cMethods
-                             (projT1 ComputationalSplitter)
-                             {| StringBound.bindex := "splits";
-                                StringBound.indexb := ?b |}]
-              => let m' := (eval simpl in (ComputationalADT.cMethods
-                                             (projT1 ComputationalSplitter)
-                                             {| StringBound.bindex := "splits";
-                                                StringBound.indexb := b |})) in
-                 change ((ComputationalADT.cMethods
-                            (projT1 ComputationalSplitter)
-                            {| StringBound.bindex := "splits";
-                               StringBound.indexb := b |}))
-                 with m' in impl
-          end).
-  Timeout 2 (repeat (let impl' := (eval cbv delta [impl] in impl) in
-          match impl' with
-            | appcontext G[ComputationalADT.cMethods
-                             (projT1 ComputationalSplitter)
-                             {| StringBound.bindex := "is_char";
-                                StringBound.indexb := ?b |}]
-              => let m' := (eval simpl in (ComputationalADT.cMethods
-                                             (projT1 ComputationalSplitter)
-                                             {| StringBound.bindex := "is_char";
-                                                StringBound.indexb := b |})) in
-                 change ((ComputationalADT.cMethods
-                            (projT1 ComputationalSplitter)
-                            {| StringBound.bindex := "is_char";
-                               StringBound.indexb := b |}))
-                 with m' in impl
-          end)).
-  Timeout 2 cbv beta iota zeta in impl.
-  Timeout 2 (do 6 let impl' := (eval cbv delta [impl] in impl) in
-                    match impl' with
-                      | appcontext G[fst (?x, ?y)] => change (fst (x, y)) with x in impl
-                      | appcontext G[snd (?x, ?y)] => change (snd (x, y)) with y in impl
-                    end).
-  Opaque ComputationalSplitter.
-  Timeout 2 simpl in impl.
-  Timeout 5 (let impl' := (eval cbv delta [impl] in impl) in
-          match impl' with
-            | appcontext G[fst (?x, _)] => let G' := context G[x] in pose G'
-            | appcontext G[snd (_, ?x)] => let G' := context G[x] in change impl' with G' in impl
-          end).
-  Timeout 5 (let impl' := (eval cbv delta [impl] in impl) in
-                    match impl' with
-                      | appcontext G[fst (?x, ?y)] => timeout 2 change (fst (x, y)) with x in impl
-                      | appcontext G[snd (?x, ?y)] => timeout 2 change (snd (x, y)) with y in impl
-                    end).
-
-  Timeout 2 simpl in c.
-               | appcontext G[snd (_, ?x)] => let G' := context G[x] in change impl' with G' in impl
-             end).
-
-  match
-  Timeout 4 do_simpl_in (projT1 ComputationalSplitter) impl.
-  Arguments SplitterFromParserADT.mis_char / .
-    change (splits_for
-                         (SplitterFromParserADT.adt_based_splitter
-                            ComputationalSplitter)) with sf in impl.
-
-  Timeout 2 simpl in impl.
-  Timeout 2 cbv beta iota zeta delta [List.map] in impl.
-
-  Timeout 2 hnf in sf.
-  let T := match type of sf with ?T -> _ => constr:T end in
-  set (T' := T) in sf;
-    change T with T' in sf.
-  match eval cbv delta [sf] in sf with
-    | fun x : ?T => _ => change T with T' in sf
-  end.
-  Timeout 2 simpl in sf.
-  Timeout 2 cbv delta [sf] in impl.
-  subst T' sf.
-  Timeout 2 change
-  Timeout 2 simpl in sf.
-  Timeout 2 let term := constr:() in
-  let term' := (eval simpl in term) in
-  let term'' := (eval cbv beta in (fun str : { r : (String.string * (nat * nat)) | exists orig, AbsR (projT2 ComputationalSplitter) orig r }%type => term' str)) in
-  idtac.
-  change term with term'' in impl.
-  change term with
-Local Ltac do_simpl_in term hyp :=
-  let term' := (eval simpl in term) in
-  change term with term' in hyp.
-
-  Timeout 2 do_simpl_in () impl.
-assert (x : { r : (String.string * (nat * nat)) | exists orig, AbsR (projT2 ComputationalSplitter) orig r }%type) by (exfalso; clear; admit).
-pose (splits_for
-                                              (SplitterFromParserADT.adt_based_splitter
-                                                 ComputationalSplitter) x).
-Timeout 2 simpl in l.
-
-Timeout 2 simpl in l.
-
-  Timeout 2 simpl @fst in impl.
-
-  match goal with
-    | [
-  Timeout 2 unfold List.fold_right in impl.
-  Timeout 2 unfold BooleanRecognizer.parse_production in impl.
-  Timeout 2 simpl BooleanRecognizer.parse_production in impl.
-  cbv beta iota zeta delta [string_has_parse ParserInterface.has_parse base_parser ParserImplementation.parser BooleanRecognizer.parse_nonterminal BooleanRecognizer.parse_nonterminal_or_abort BooleanRecognizer.parse_nonterminal_step BooleanRecognizer.parse_productions BaseTypes.initial_nonterminals_data BooleanBaseTypes.predata ParserImplementation.parser_data RDPList.rdp_list_predata BaseTypes.remove_nonterminal BaseTypes.nonterminals_listT_R BaseTypes.nonterminals_listT RDPList.rdp_list_nonterminals_listT RDPList.rdp_list_nonterminals_listT_R BaseTypes.is_valid_nonterminal RDPList.rdp_list_is_valid_nonterminal BaseTypes.ntl_wf RDPList.rdp_list_remove_nonterminal] in impl.
-  Timeout 2 do_simpl_in (Lookup ab_star_grammar) impl.
-  Timeout 2 cbv beta iota zeta in impl.
-  let impl' := (eval cbv delta [impl] in impl) in exact impl'.
-Defined.
-
-Definition ab_star_parser : String.string -> bool
-  := Eval cbv zeta delta [ab_star_parser'] in ab_star_parser'.
-Require Import ExtrOcamlBasic.
-Require Import ExtrOcamlString.
-Require Import ExtrOcamlIntConv.
-Require Import ExtrOcamlNatInt.
 Recursive Extraction ab_star_parser.
-Proof.
-
-
-  Timeout 5 simpl in impl.
-
-
-
-  cbv beta iota zeta delta [Wf.Fix3] in impl.
-  Timeout 2 change ((@StringLike.length _ (ParserInterface.string_type
-                                             (SplitterFromParserADT.adt_based_splitter
-                                                ComputationalSplitter))))
-  with (fun str : { r : (String.string * (nat * nat)) | exists orig, AbsR (projT2 ComputationalSplitter) orig r }%type => ilength (` str)) in impl.
-  Timeout 2 change (@StringLike.length  _ (ParserInterface.string_type
-                                                (SplitterFromParserADT.adt_based_splitter
-                                                   ComputationalSplitter)))
-  with (fun str :
-  with (fun str : {r : string * (nat * nat) | hextr0} =>
-        SplitterFromParserADT.mlength ComputationalSplitter () (` str))
-  in impl"), last call failed.
-  Timeout 2 do_simpl_in (@StringLike.length _ (ParserInterface.string_type
-                                                (SplitterFromParserADT.adt_based_splitter
-                                                   ComputationalSplitter))) impl.
-
-  with (exist _ (str, (0, String.length str)) (proj2_sig (new_string_of_base_string ComputationalSplitter str))) in impl.
-  Arguments new_string_of_base_string / .
-
-  Timeout 2 do_simpl_in (new_string_of_base_string ComputationalSplitter str) impl.
-
-  Timeout 2 lazy beta iota zeta delta [BaseTypes.remove_nonterminal BaseTypes.nonterminals_listT_R StringLike.String StringLike.length] in impl.
-  unfold Lookup in *.
-
-  unfold RelationClasses.reflexivity in impl.
-  unfold RelationClasses.Equivalence_Reflexive in impl.
-  unfold bool_eq_Equivalence in *.
-  Timeout 3 cbv delta [BooleanRecognizer.parse_nonterminal BooleanRecognizer.parse_nonterminal_or_abort] in b.
-  Timeout 10 simpl in b.
-  let impl := (eval unfold b in b) in
-  let impl' := (eval cbv beta iota zeta delta [BooleanRecognizer.parse_nonterminal] in impl) in
-  pose impl'.
-Timeout 2 simpl in b.
-  refine (fun s => has_parse (parser (adt_based_splitter ComputationalSplitter))
-                             (exist _ (cConstructors (projT1 ComputationalSplitter) {| StringBound.bindex := "new" |} s) (ex_intro _ s _))).
-  abstract (
-      pose proof (ADTRefinementPreservesConstructors (projT2 ComputationalSplitter) {| StringBound.bindex := "new" |} s (cConstructors (projT1 ComputationalSplitter) {| StringBound.bindex := "new" |} s) (ReturnComputes _)) as H'';
-      computes_to_inv;
-      simpl in H'';
-      computes_to_inv; subst; assumption
-    ).
-Defined.
-
-Definition ab_star_parser' : String.string -> bool.
-Proof.
-Print ab_star_parser.
-
-
-  hnf.
-  simpl.
-  simpl.
-  pose .
-  simpl in *.
-  Require Import StringLike.Core StringLike.String.
-  Timeout 2 simpl.
-  hnf.
-  unfold string_type.
-  Locate adt_based_splitter.
-  pose .
-  simpl in c.
-  unfold cConstructorType in *.
-
-lazy.
- (s, (0, String.length s))).
-    simpl in b.
-Require Import StringLike.Core.
-simpl in b.
-Set Printing All.
-
-
-Check ab_star_parser.
-Check .
